Neue alte Tape-Kodierung

TM/Code/FinTM.v
@@ -11,35 +11,35 @@ Section FinTM1.
   Let sig' := sig' sig.
 
   Definition UnaryFinTM : { M : mTM sig' 1 & states M -> unit } :=
-    TapeInit sig ;;
-             MATCH (Read_char _)
-             (fun r1 =>
-                match r1 with
-                | Some (inl r1') => Write (inl (f r1')) tt
-                | _ => mono_Nop _ tt
-                end).
+    MATCH (Read_char _)
+          (fun r1 =>
+             match r1 with
+             | Some (inl r1') => Write (inl (f r1')) tt
+             | _ => mono_Nop _ tt
+             end).
   
   Lemma UnaryFinTM_Computes :
-    UnaryFinTM ⊨ Computes_Rel Fin.F1 Fin.F1 cX cX f.
+    UnaryFinTM ⊨c(3) Computes_Rel Fin.F1 Fin.F1 cX cX f.
   Proof.
-    eapply Realise_monotone.
-    - unfold UnaryFinTM. eapply Seq_Realise.
-      + eapply TapeInit_Realise with (X := sig) (cX := cX).
-      + eapply Match_Realise.
-        * eapply RealiseIn_Realise. eapply read_char_sem.
-        * instantiate (1 := fun r1 => match r1 with Some (inl r1') => _ | _ => _ end).
-          intros y. cbn in y. destruct y as [ [ | ] | ]; cbn in *.
-          -- eapply RealiseIn_Realise. eapply Write_Sem.
-          -- eapply RealiseIn_Realise. eapply mono_Nop_Sem.
-          -- eapply RealiseIn_Realise. eapply mono_Nop_Sem.
-    - hnf. intros tin (yout, tout). intros H. hnf in H. destruct H as ((y1&t1)&H1&H2). hnf in *.
-      destruct H2 as (r1&t2&(He1&He2)&H3); hnf in *; subst. intros x (r1&r2&EncX). specialize (H1 _ _ _ EncX) as (H1&H2).
-      cbn in *. pose proof tape_local_current_cons H2 as H2'. destruct_tapes. cbn in *. rewrite H2' in H3. hnf in H3.
-      destruct H3 as (_&H3). cbn in *. subst. destruct yout, y1.
-      unfold sig', CodeTM.sig', finType_CS in *. cbn in *. hnf in EncX.
-      rewrite H1. hnf. do 2 eexists. hnf. cbn. simpl_list.
-      instantiate (1 := r2). instantiate (1 := r1). f_equal. cbn. f_equal. f_equal. 
-      erewrite tape_local_right; eauto.
+    eapply RealiseIn_monotone.
+    - unfold UnaryFinTM. eapply Match_RealiseIn.
+      + eapply read_char_sem.
+      + instantiate (2 := fun r1 => match r1 with Some (inl r1') => _ | _ => _ end).
+        intros y. cbn in y. destruct y as [ [ | ] | ]; cbn in *.
+        * eapply Write_Sem.
+        * eapply mono_Nop_Sem.
+        * eapply mono_Nop_Sem.
+    - cbn. omega.
+    - hnf. intros tin (yout, tout) H x (r1&r2&H3&H4). hnf in H.
+      destruct H as (y&t2&H1&H2). hnf in *. destruct y as [ [ | ] | ]; hnf in *.
+      + (* valid input *) destruct H1 as (H&H'). hnf in *. destruct H2 as (->&H2). subst.
+        destruct_tapes. cbn in *. subst. cbn.
+        pose proof tape_local_current_cons H4 as H4'; rewrite H4' in H; inv H; clear H4'.
+        do 2 eexists. hnf; cbn. split; eauto. f_equal. eapply tape_local_right; eauto.
+      + (* invalid input *) destruct H1 as (H&H'). hnf in *. destruct H2 as (->&->). subst. cbn in *.
+        apply tape_local_current_cons in H4. destruct_tapes. cbn in *. congruence.
+      + (* invalid input *) destruct H1 as (H&H'). hnf in *. destruct H2 as (->&->). subst. cbn in *.
+        apply tape_local_current_cons in H4. destruct_tapes. cbn in *. congruence.
   Qed.
   
 End FinTM1.
